Foundation/FirstOrder/Arithmetic/PA/Prenex.lean
@@ -6,7 +6,7 @@ public import Foundation.FirstOrder.Arithmetic.StrictEquiv
 # Prenex normal form theorem over $\mathsf{PA}$
 
 Every `Hierarchy Γ s` formula is `𝗣𝗔`-provably equivalent to an alternating quantifier prefix
-over a bounded kernel.
+over a bounded matrix.
 -/
 
 @[expose] public section
@@ -18,29 +18,29 @@ namespace LO.FirstOrder.Arithmetic.Peano
 
 variable {Γ : Polarity} {s n : ℕ}
 
-lemma nonempty_strictHierarchyFormulaEquivOf {φ : ArithmeticSemisentence n} (h : Hierarchy Γ s φ) :
-    Nonempty (StrictHierarchyFormulaEquivOf 𝗣𝗔 Γ s φ) :=
-  Arithmetic.nonempty_strictHierarchyFormulaEquivOf h
+lemma nonempty_prenexEquivOf {φ : ArithmeticSemisentence n} (h : Hierarchy Γ s φ) :
+    Nonempty (PrenexEquivOf 𝗣𝗔 Γ s _ φ) :=
+  Arithmetic.nonempty_prenexEquivOf h
 
-lemma exists_kernel_provable {φ : ArithmeticSemisentence n} (h : Hierarchy Γ s φ) :
+lemma exists_matrix_provable {φ : ArithmeticSemisentence n} (h : Hierarchy Γ s φ) :
     ∃ φ₀ : ArithmeticSemisentence (n + s),
       Hierarchy 𝚺 0 φ₀ ∧ 𝗣𝗔 ⊢ ∀¹* (φ 🡘 Polarity.quantItr Γ s φ₀) := by
-  obtain ⟨φ'⟩ := nonempty_strictHierarchyFormulaEquivOf h;
-  exact ⟨φ'.kernel, φ'.kernel_deltaZero, φ'.provable⟩
+  obtain ⟨φ'⟩ := nonempty_prenexEquivOf h;
+  exact ⟨φ'.matrix, φ'.toPrenex.matrix_Δ₀, φ'.provable⟩
 
-lemma exists_kernel_provable_of_sentence {σ : ArithmeticSentence} (h : Hierarchy Γ s σ) :
+lemma exists_matrix_provable_of_sentence {σ : ArithmeticSentence} (h : Hierarchy Γ s σ) :
     ∃ π₀ : ArithmeticSemisentence (0 + s),
       Hierarchy 𝚺 0 π₀ ∧ 𝗣𝗔 ⊢ σ 🡘 Polarity.quantItr Γ s π₀ :=
-  exists_kernel_provable h
+  exists_matrix_provable h
 
 lemma exists_hierarchy_provable_of_sentence {σ : ArithmeticSentence} (h : Hierarchy 𝚺 (s + 1) σ) :
     ∃ θ : ArithmeticSemisentence 1, Hierarchy 𝚷 s θ ∧ 𝗣𝗔 ⊢ σ 🡘 ∃¹ θ := by
-  obtain ⟨σ'⟩ := nonempty_strictHierarchyFormulaEquivOf h;
+  obtain ⟨σ'⟩ := nonempty_prenexEquivOf h;
   exact ⟨↑σ'.sigmaInv, σ'.sigmaInv.hierarchy, σ'.provable_sigmaInv⟩
 
 lemma exists_hierarchy_provable_of_sentence_pi {σ : ArithmeticSentence} (h : Hierarchy 𝚷 (s + 1) σ) :
     ∃ θ : ArithmeticSemisentence 1, Hierarchy 𝚺 s θ ∧ 𝗣𝗔 ⊢ σ 🡘 ∀¹ θ := by
-  obtain ⟨σ'⟩ := nonempty_strictHierarchyFormulaEquivOf h;
+  obtain ⟨σ'⟩ := nonempty_prenexEquivOf h;
   exact ⟨↑σ'.piInv, σ'.piInv.hierarchy, σ'.provable_piInv⟩
 
 end LO.FirstOrder.Arithmetic.Peano
